Given an expression \( f(x) = x^2+5 \), the derivative, \( f'(x) \), from first principle is given by:

\begin{align}
    f'(x) &= \lim_{\delta x \to 0}
        \frac{
            f(x + \delta x) - f(x)
        }{ \delta x }
    \\
    &= \lim_{\delta x \to 0}
        \frac{
            {(x + \delta x)}^2+5 - (x^2+5)
        }{ \delta x }
    \nonumber \\
    &= \lim_{\delta x \to 0}
        \frac{
            x^2 + 2x\delta x + {\delta x}^2 +5 - (x^2+5)
        }{ \delta x }
    \nonumber \\
    &= \lim_{\delta x \to 0}
        \frac{
            \cancel{\delta x} (2x + \delta x)
        }{ \cancel{\delta x} }
    \nonumber \\
    f'(x) &= 2x 
\end{align}
